TargetSFI/CSTest.v
@@ -1,11 +1,71 @@
 Require Import TargetSFI.CS.
+Require Import TargetSFI.Machine.
+Require Import TargetSFI.MachineGen.
+Require Import Coq.Lists.List. Import ListNotations.
+Require Import Coq.Logic.Decidable.
+
+From QuickChick Require Import QuickChick.
+Import QcDefaultNotation. Import QcNotation. Open Scope qc_scope.
+Import GenLow GenHigh.
+(* Suppress some annoying warnings: *)
+Set Warnings "-extraction-opaque-accessed,-extraction".
+
+Require Import CompCert.Events.
 
 Import CS.
+Import Env.
+Import RiscMachine.
+Import RiscMachine.ISA.
 
 
-  (* Definition eval_step_complete : Prop := *)
-  (*   forall (G : Env.t)  (st : MachineState.t) (t : trace) (st' : MachineState.t), *)
-  (*     (step G st t st') -> (eval_step G st = Some (t, st')). *)
+Instance executing_dec (mem : RiscMachine.Memory.t) (pc : RiscMachine.address)
+         ( i : RiscMachine.ISA.instr) : Dec (executing mem pc i).
+Proof.
+  apply Build_Dec. unfold ssrbool.decidable.
+  unfold executing.
+  destruct ( Memory.get_word mem pc0).
+  - destruct w.
+    + auto.
+    + apply instr_eq_dec.
+  - auto.
+Defined.
+    
+Instance step_dec(g : Env.t) (st : MachineState.t) (t : trace)
+         (st' : MachineState.t): Dec (step g st t st'). 
+Proof.
+  apply Build_Dec. unfold ssrbool.decidable.
+  destruct st as [[mem pc] gen_regs].
+  destruct st' as [[mem' pc'] gen_regs'].
+  destruct (Memory.get_word mem pc) eqn:H.
+  - destruct w.
+    + right. unfold not. intro H1.
+      (* TODO Learn how to write a tactic pattern here to match all the cases
+      inversion H1; try (unfold executing in H5; subst; rewrite H in H5; auto).
+      * *)
+      Admitted.
+
+Definition trace_checker (t1 t2 : trace) : Checker := checker true. (* TODO *)
+
+Definition state_checker (s1 s2: MachineState.t) : Checker := checker true. (* TODO *)
+
+Definition eval_step_complete_exec : Checker :=
+  forAll genEnv (fun g =>
+  forAll (genStateForEnv g) (fun st =>
+  forAll (genTrace g st) (fun t =>
+  forAll (genNextState g st t)
+         (fun st' =>
+            if (step g st t st')?
+            then
+              match (eval_step g st) with
+              | Some (t1,st1) =>
+                conjoin [ (trace_checker t1 t); (state_checker st' st1) ]
+              | None =>
+                checker false
+              end
+            else checker true (* at some point I want to have some incorrect cases to test *)
+         )))).
+              
+                                                            
 
 (*
 What do I need to generate?
